...역시, 여기서 막히네. 뭐 제대로 증명 되는 게 없어...!

src/study/Nemonuri.Study.CSharpSyntaxRewriter2.Modifier2/Nemonuri.StratifiedNodes.Nodes.Base.Members.fst
@@ -6,6 +6,39 @@ module T = Nemonuri.StratifiedNodes.Nodes.Base.Types
 module Math = FStar.Math.Lib
 open FStar.Classical.Sugar
 
+//--- (T.node_list_index t) or (T.option_node_list_index t) members ---
+
+let is_node_list_index #t (index:nat) (node_list:T.node_list t) 
+  : Tot bool =
+  (Cons? node_list) && (index < (L.length node_list))
+
+let is_not_node_list_index #t (index:nat) (node_list:T.node_list t) 
+  : Tot bool =
+  (Nil? node_list) || (index >= (L.length node_list))
+
+private let _ = assert ( forall t index node_list .
+  (is_node_list_index #t index node_list) \/
+  (is_not_node_list_index #t index node_list)
+ )
+
+let try_convert_to_node_list_index #t (index:nat) (node_list:T.node_list t) 
+  : Pure (T.option_node_list_index node_list) True
+    (ensures fun r ->
+      match r with
+      | Some v1 -> (is_node_list_index index node_list) && (v1 = index)
+      | None -> is_not_node_list_index index node_list
+    )
+  =
+  match is_node_list_index index node_list with
+  | true -> Some index
+  | false -> None //<: (T.option_node_list_index node_list)
+
+let is_node_list_index_list #t (l:list nat) (node_list:T.node_list t)
+  : Tot bool =
+  L.for_all (fun (index:nat) -> is_node_list_index index node_list) l 
+
+//---|
+
 //--- (T.node t) members ---
 let get_level #t (node:T.node t) 
   : Pure pos True (ensures fun r -> (r = (I.get_level node.internal)))
@@ -20,6 +53,45 @@ private let rec get_list_level_impl #t (l:T.node_list t) : Tot nat =
   match l with
   | [] -> 0
   | hd::tl -> Math.max (get_level hd) (get_list_level_impl tl)
+
+(*
+private let rec get_index_list_from_predicate_core #t 
+  (node_list:T.node_list t) (predicate: (T.node t) -> Tot bool)
+  : Tot (nat & (list nat))
+    (decreases node_list)
+  =
+  match node_list with
+  | [] -> (0, [])
+  | hd::tl ->
+  let (reverse_index, satisfied_reverse_index_list) = get_index_list_from_predicate_core tl predicate in
+  let next_reverse_index = reverse_index + 1 in
+  let next_satisfied_reverse_index_list = (if (predicate hd) then (reverse_index::satisfied_reverse_index_list) else satisfied_reverse_index_list ) in
+  ( reverse_index, next_satisfied_reverse_index_list )
+*)
+
+private let rec get_index_list_from_predicate_impl_core #t 
+  (node_list: T.node_list t) (predicate: (T.node t) -> Tot bool) 
+  (current_index: nat) (current_index_list: list nat)
+  : Tot (list nat) 
+    (decreases node_list)
+  =
+  match node_list with
+  | [] -> current_index_list
+  | hd::tl -> 
+  let next_lndex_list = (
+    match (predicate hd) with
+    | true -> current_index::current_index_list
+    | false -> current_index_list
+  ) in
+  get_index_list_from_predicate_impl_core 
+    tl predicate (current_index + 1) next_lndex_list
+
+private let get_index_list_from_predicate_impl #t
+  (node_list: T.node_list t) (predicate: (T.node t) -> Tot bool) 
+  : Tot (list nat) =
+  get_index_list_from_predicate_impl_core 
+    node_list predicate 0 []
+
 //---|
 
 //--- (T.node_list t) propositions ---
@@ -28,6 +100,12 @@ let list_level_is_greater_or_equal_than_any_element_level
   : prop =
   (forall (node:T.node t). 
     (L.contains node l) ==> ((get_level node) <= get_list_level_impl l))
+
+let result_of_get_index_list_from_predicate_is_node_list_index_list #t
+  (node_list: T.node_list t) (predicate: (T.node t) -> Tot bool) 
+  : prop =
+  let v0 = get_index_list_from_predicate_impl node_list predicate in
+  is_node_list_index_list v0 node_list
 //---|
 
 //--- (T.node_list t) lemmas ---
@@ -63,6 +141,35 @@ let get_list_level #t (l:T.node_list t)
   lemma_list_level_is_greater_or_equal_than_any_element_level t l;
   get_list_level_impl l
 
+let get_item #t (node_list:T.node_list t) (index:T.node_list_index node_list)
+  : Tot (T.node t)
+  =
+  L.index node_list index
+
+let try_get_item #t (node_list:T.node_list t) (index:nat)
+  : Tot (option (T.node t))
+  =
+  match try_convert_to_node_list_index index node_list with
+  | Some v1 -> Some (get_item node_list v1)
+  | None -> None
+
+(*
+let rec get_index_list_from_predicate #t 
+  (node_list:T.node_list t) (predicate: (T.node t) -> Tot bool)
+  : Pure (list nat) True
+    (ensures fun r ->
+      forall (index_in_result:nat). (L.contains index_in_result node_list) ==>
+      ((is_node_list_index index_in_result node_list) /\
+       (predicate (L.index node_list index_in_result))
+      )
+    )
+    (decreases node_list)
+  =
+  match node_list with
+  | [] -> []
+  | hd::tl ->
+*)
+
 let rec try_get_first_index_of_predicate #t 
   (node_list:T.node_list t) (predicate: (T.node t) -> Tot bool)
   : Pure (option nat) True
@@ -82,4 +189,24 @@ let rec try_get_first_index_of_predicate #t
   match try_get_first_index_of_predicate tl predicate with
   | None -> None
   | Some v1 -> Some (1 + v1)
+
+let get_index_list_from_predicate #t
+  (node_list: T.node_list t) (predicate: (T.node t) -> Tot bool)
+  : Pure (list nat) True
+    (ensures fun r -> 
+      result_of_get_index_list_from_predicate_is_node_list_index_list node_list predicate)
+  =
+  assume (result_of_get_index_list_from_predicate_is_node_list_index_list node_list predicate);
+  get_index_list_from_predicate_impl node_list predicate
+
+(*
+private let _ = assert ( forall t node_list predicate.
+  let r = get_index_list_from_predicate #t node_list predicate in
+  ( forall index_in_result. 
+      (L.contains index_in_result r) ==>
+        ((is_node_list_index index_in_result node_list) /\
+        (predicate (L.index node_list index_in_result)) )
+  )
+)
+*)
 //---|
