src/study/Nemonuri.Study.CSharpSyntaxRewriter2.Modifier2/Nemonuri.StratifiedNodes.Factories.NodeLists.fst
@@ -88,7 +88,6 @@ let replace_range_at #t
   let v1 = remove_at node_list index in
   insert_range node_list index inserting_node_list
 
-
 let replace_range #t
   (node_list:N.node_list t) 
   (node:N.node t) //{ L.contains node node_list }
@@ -99,5 +98,12 @@ let replace_range #t
   let Some index = N.try_get_first_index_of_predicate node_list (op_Equality node) in
   replace_range_at node_list index inserting_node_list
 
+let replace #t
+  (node_list:N.node_list t) 
+  (node:N.node t) //{ L.contains node node_list }
+  (inserting_node:N.node t)
+  : Tot (N.node_list t)
+  =
+  replace_range node_list node [inserting_node]
 
 //---|
